lnBreak;
​
// Approach - 2(i) --> Recursive --> T.C - O(N), S.C - O(N)
print(head2);
cout << head2 -> data << " ";
cout << tail2 -> data << ln;
​
reverseLinkedListRecursive1(head2, tail2);
​
print(head2);
cout << head2 -> data << " ";
cout << tail2 -> data << ln;
​
lnBreak;
​
// Approach - 2(ii) --> Recursive --> T.C - O(N), S.C - O(N)
print(head2);
cout << head2 -> data << " ";
cout << tail2 -> data << ln;
​
reverseLinkedListRecursive2(head2, tail2);
​
print(head2);
cout << head2 -> data << " ";
cout << tail2 -> data << ln;
​
lnBreak;
}
​
```